new/proof/github_com/sanjit_bhat/pav/merkle_proof/base.v
@@ -15,6 +15,8 @@ Notation cutNodeTy := (W8 0) (only parsing).
 Notation leafNodeTy := (W8 1) (only parsing).
 Notation innerNodeTy := (W8 2) (only parsing).
 
+Notation max_depth := 256%nat.
+
 Section proof.
 Context `{hG: heapGS Σ, !ffi_semantics _ _, !goGlobalsGS Σ}.
 Context `{!ghost_varG Σ ()}.
